fix subst_map_rel: take 'context' and require all its variables to be in the map

theories/simplang/open_expr_rel.v
@@ -5,58 +5,66 @@ From simuliris.simulation Require Import slsls lifting.
 From simuliris.simplang Require Import proofmode tactics.
 From simuliris.simplang Require Import parallel_subst heap_bij.
 
-(** map_ForallI *)
-Definition map_ForallI `{Lookup K A M} `(P : K → A → iProp Σ) : M → iProp Σ :=
-    (λ m, ∀ i x, ⌜m !! i = Some x⌝ → P i x)%I.
-Section map_Forall.
-  Context `{FinMap K M}.
-  Context {A} {Σ} (P : K → A → iProp Σ).
-  Implicit Types m : M A.
-
-  Lemma map_ForallI_empty : ⊢ map_ForallI P (∅ : M A).
-  Proof. iIntros (i x). rewrite lookup_empty. by iIntros "%". Qed.
-  Lemma map_ForallI_insert_2 m i x :
-    ⊢ P i x -∗ map_ForallI P m -∗ map_ForallI P (<[i:=x]>m).
-  Proof.
-    iIntros "? Hm" (j y); rewrite lookup_insert_Some.
-    iIntros "%Hv". destruct Hv as [[-> ->] | [Hneq Hs]]; first done.
-    by iApply "Hm".
-  Qed.
-End map_Forall.
-
 Section open_rel.
   Context `{sbijG Σ}.
 
-  (** Well-formed substitutions in source and target*)
+  (** Well-formed substitutions closing source and target, with [X] denoting the
+      free variables. *)
+  Definition subst_map_rel (X : gset string) (map : gmap string (val * val)) : iProp Σ :=
+    [∗ set] x ∈ X,
+      match map !! x with
+      | Some (v_t, v_s) => val_rel v_t v_s
+      | None => False
+      end.
 
-  Definition subst_map_rel (map : gmap string (val * val)) :=
-    map_ForallI (λ _ '(v_t, v_s), val_rel v_t v_s) map.
-
-  Global Instance subst_map_rel_pers map : Persistent (subst_map_rel map).
+  Global Instance subst_map_rel_pers X map : Persistent (subst_map_rel X map).
   Proof.
-    rewrite /subst_map_rel /map_ForallI.
-    apply bi.forall_persistent => x. apply bi.forall_persistent; intros [a b].
-    apply _.
+    rewrite /subst_map_rel. apply big_sepS_persistent=>x.
+    destruct (map !! x) as [[v_t v_s]|]; apply _.
   Qed.
 
-  Lemma subst_map_rel_insert map v_t v_s b :
+  Lemma subst_map_rel_lookup {X map} x :
+    x ∈ X →
+    subst_map_rel X map -∗
+    ∃ v_t v_s, ⌜map !! x = Some (v_t, v_s)⌝ ∗ val_rel v_t v_s.
+  Proof.
+    iIntros (Hx) "Hrel".
+    iDestruct (big_sepS_elem_of _ _ x with "Hrel") as "Hrel"; first done.
+    destruct (map !! x) as [[v_t v_s]|]; last done. eauto.
+  Qed.
+
+  Lemma subst_map_rel_weaken {X1} X2 map :
+    X2 ⊆ X1 →
+    subst_map_rel X1 map -∗ subst_map_rel X2 map.
+  Proof. iIntros (HX). iApply big_sepS_subseteq. done. Qed.
+
+  (* TODO: use [binder_delete], once we can [delete] on [gset]. *)
+  Definition binder_delete_gset (b : binder) (X : gset string) :=
+    match b with BAnon => X | BNamed x => X ∖ {[x]} end.
+
+  Lemma subst_map_rel_insert X x v_t v_s map :
+    subst_map_rel (binder_delete_gset x X) map -∗
     val_rel v_t v_s -∗
-    subst_map_rel map -∗
-    subst_map_rel (binder_insert b (v_t, v_s) map).
+    subst_map_rel X (binder_insert x (v_t, v_s) map).
   Proof.
-    iIntros "Hv Hs". destruct b; first done. by iApply (map_ForallI_insert_2 with "[Hv] Hs").
+    iIntros "#Hmap #Hval". destruct x; first done. simpl.
+    iApply big_sepS_intro. iIntros "!# %s' %Hs'".
+    destruct (decide (s = s')) as [->|Hne].
+    - rewrite lookup_insert. done.
+    - rewrite lookup_insert_ne //.
+      iApply (big_sepS_elem_of with "Hmap"). set_solver.
   Qed.
 
-  Lemma subst_map_rel_empty : ⊢ subst_map_rel ∅.
-  Proof. apply map_ForallI_empty. Qed.
+  Lemma subst_map_rel_empty map :
+    ⊢ subst_map_rel ∅ map.
+  Proof. iApply big_sepS_empty. done. Qed.
 
   (** The "expression relation" of our logical relation:
       The simulation relation must hold after applying an arbitrary well-formed
       closing substitution [map]. *)
   Definition expr_rel e_t e_s : iProp Σ :=
     ∀ π (map : gmap string (val * val)),
-      ⌜free_vars e_t ∪ free_vars e_s ⊆ dom (gset _) map⌝ -∗
-      subst_map_rel map -∗
+      subst_map_rel (free_vars e_t ∪ free_vars e_s) map -∗
       subst_map (fst <$> map) e_t ⪯{π, val_rel} subst_map (snd <$> map) e_s {{ val_rel }}.
 
   Lemma expr_rel_closed e_t e_s :
@@ -67,9 +75,9 @@ Section open_rel.
     intros Hclosed_t Hclosed_s. iSplit.
     - iIntros "Hwf" (π). iSpecialize ("Hwf" $! π ∅).
       rewrite ->!fmap_empty, ->!subst_map_empty.
-      iApply "Hwf"; last by iApply subst_map_rel_empty.
-      iPureIntro. set_solver.
-    - iIntros "Hsim" (π xs _) "Hxs".
+      rewrite Hclosed_t Hclosed_s [∅ ∪ _]left_id_L.
+      iApply "Hwf". by iApply subst_map_rel_empty.
+    - iIntros "Hsim" (π xs) "Hxs".
       rewrite !subst_map_closed //.
   Qed.
 
@@ -80,18 +88,17 @@ Section open_rel.
       expr_rel (subst x v_t e_t) (subst x v_s e_s)) -∗
     expr_rel e_t e_s.
   Proof.
-    iIntros "Hsim" (π xs Hdom) "#Hxs".
+    iIntros "Hsim" (π xs) "#Hxs".
     destruct (decide (x ∈ free_vars e_t ∪ free_vars e_s)) as [Hin|Hnotin]; last first.
     { iSpecialize ("Hsim" $! #0 #0).
       rewrite ->subst_free_vars by set_solver.
       rewrite ->subst_free_vars by set_solver.
       iApply "Hsim"; eauto. }
-    assert (is_Some (xs !! x)) as [[v_t v_s] Hv].
-    { apply elem_of_dom. set_solver. }
-    iSpecialize ("Hsim" $! v_t v_s with "[]").
-    { iApply ("Hxs" $! _ (_, _)). done. }
-    iSpecialize ("Hsim" $! π xs with "[] Hxs").
-    { iPureIntro. rewrite !free_vars_subst. set_solver. }
+    iDestruct (subst_map_rel_lookup x with "Hxs") as (v_t v_s Hv) "Hrel"; first done.
+    iSpecialize ("Hsim" $! v_t v_s with "Hrel").
+    iSpecialize ("Hsim" $! π xs with "[Hxs]").
+    { iApply (subst_map_rel_weaken with "Hxs").
+      rewrite !free_vars_subst. set_solver. }
     rewrite !subst_map_subst.
     rewrite insert_id.
     2:{ rewrite lookup_fmap Hv //. }
